\documentclass{article}
\usepackage{amsmath,amsthm,amssymb,amsfonts,fullpage,fancyhdr}

\pagestyle{fancy}
\renewcommand{\headheight}{50pt}
\renewcommand{\footskip}{10pt}
\renewcommand{\textheight}{609pt}
\renewcommand{\headrulewidth}{0pt}

\newtheorem{problem}{Problem}

\begin{document}

\rhead{Kris Harper\\MATH 25800\\February 10, 2010\\}
\chead{Quiz 3\\}

\begin{problem}
If $N$ is a submodule of $M$, the \emph{annihilator of $N$ in $R$} is defined to be $\{r \in R \mid rn = 0 \text{ for all } n \in N\}$. Prove that annihilator of $N$ in $R$ is a $2$-sided ideal of $R$.
\end{problem}
\begin{proof}
Let $N$ be a submodule of $M$ and let $A$ be the annihilator of $N$ in $R$. Let $a,b \in A$ and let $n \in N$. Then $(a-b)n = an-bn = 0-0 = 0$ so $a-b \in A$ and $(ab)n = a(bn) = a \cdot 0 = 0$ since $0 \in N$ so $ab \in A$. Finally, let $r \in R$ and note that $(ra)n = r(an) = r \cdot 0 = 0$ and $(ar)n = a(rn) = 0$ since $rn \in N$. (Note that $r \cdot 0 = 0$ follows from the usual proof---$r \cdot 0 = r(0 + 0) = r \cdot 0 + r \cdot 0$ so $0 = r \cdot 0$). Since $a$, $b$, $n$ and $r$ are arbitrary, this shows that $A$ is subring of $R$ which is closed under left and right multiplication by elements in $R$. Therefore $A$ is $2$-sided ideal of $R$.
\end{proof}

\begin{problem}
Let $N$ be a submodule of $M$. Prove that if both $M/N$ and $N$ are finitely generated then so is $M$.
\end{problem}
\begin{proof}
Suppose $M/N = RA$ and $N = RB$ where $A$ and $B$ are finite with $|A| = i$ and $|B| = j$. Let $m \in M$ and note that
\begin{align*}
\{m + n \mid n \in N\}
&= m+N\\
&= r_1(a_1 + N) + r_2(a_2 + N) + \dots + r_i(a_i + N)\\
&= ((r_1a_1) + N) + ((r_2a_2) + N) + \dots + ((r_ia_i) + N)\\
&= (r_1a_1 + r_2a_2 + \dots + r_ia_i) + N\\
&= \{(r_1a_1 + r_2a_2 + \dots + r_ia_i) + n \mid n \in N\}.
\end{align*}
So for some $n$ and $n'$ and elements of $R$ we have $m + n = (r_1a_1 + r_2a_2 + \dots + r_ia_i) + n'$. But $N$ is finitely generated by $B$, so for some other coefficients from $R$ we have
\[
m + (s_1b_1 + s_2b_2 + \dots + s_jb_j) = (r_1a_1 + r_2a_2 + \dots + r_ia_i) + (t_1b_1 + t_2b_2 + \dots + t_jb_j)
\]
and
\[
m = r_1a_1 + r_2a_2 + \dots + r_ia_i + (t_1-s_1)b_1 + (t_2-s_2)b_2 + \dots + (t_j-s_j)b_j.
\]
So an arbitrary element of $m$ can be written as a finite sum of elements with coefficients from $R$. Thus $M$ is finitely generated.
\end{proof}

\end{document}